- Tweaked the closure conversion relation at closure_conversion.v - Progress in closure conversion proof at closure_conversion_correct.v (two cases remain) - Minor fixes in lemmas at cps_util.v

theories/L6_PCPS/closure_conversion_correct.v
@@ -323,6 +323,7 @@ Proof.
     intros. inv H0.
 Qed.
 
+
 (* Fixpoint ctx_as_env (rho : env) v C : env := *)
 (*   match C with *)
 (*     | Hole_c => rho *)
@@ -430,6 +431,470 @@ Proof.
   - eauto.
 Qed.
 
+
+Inductive ctx_to_rho : exp_ctx -> env -> env -> Prop :=
+| Hole_c_to_rho :
+    forall rho,
+      ctx_to_rho Hole_c rho rho
+| Eproj_c_to_rho :
+    forall rho rho' tau t y tau' N Γ C vs v,
+      M.get Γ rho = Some (Vconstr tau t vs) ->
+      nthN vs N = Some v ->
+      ctx_to_rho C (M.set y v rho) rho' ->
+      ctx_to_rho (Eproj_c y tau' N Γ C) rho rho'
+| Econstr_c_to_rho :
+    forall rho rho' tau t y  x Γ C v1 v2,
+      M.get Γ rho = Some v1 ->
+      M.get x rho = Some v2 ->
+      ctx_to_rho C (M.set y (Vconstr tau t [v2; v1]) rho) rho' ->
+      ctx_to_rho (Econstr_c y tau t [x; Γ] C) rho rho'.
+
+  
+Lemma project_var_correct k rho1 rho2 rho2'
+      Scope Funs Γ FVs x x' C S S'  :
+  project_var Scope Funs Γ FVs S x x' C S' ->
+  cc_approx_env_P Scope k rho1 rho2 ->
+  Fun_inv k rho1 rho2 Scope Funs Γ ->
+  env_inv k rho1 rho2 Scope Funs Γ FVs ->
+  ctx_to_rho C rho2 rho2' ->
+  Disjoint _ S (Union var Scope
+                      (Union var Funs
+                             (Union var (FromList FVs) (Singleton var Γ)))) ->
+  ~ In _ S' x' /\
+  cc_approx_env_P Scope k rho1 rho2' /\
+  Fun_inv k rho1 rho2' Scope Funs Γ /\
+  env_inv k rho1 rho2' Scope Funs Γ FVs /\
+  cc_approx_var_env k rho1 rho2' x x'.
+Proof.
+  intros Hproj Hcc Hfun Henv Hctx Hd.
+  inv Hproj. 
+  - inv Hctx. repeat split; eauto. intros Hc. eapply Hd; eauto.
+  - inv Hctx. inv H12.
+    repeat split; eauto.
+    + intros Hc. inv Hc. eauto.
+    + eapply cc_approx_env_P_set_not_in_P_r. eassumption.
+      constructor. intros y Hc. eapply Hd.
+      inv Hc. inv H3. eauto. 
+    + (* TODO : make lemma *)
+      edestruct Hfun as [tau' [t' [vs' [Hget Hfun']]]].
+      rewrite Hget in H10; inv H10.
+      do 3 eexists. rewrite M.gso; [ | now intros Heq; subst; eapply Hd; eauto ].
+      split; eauto. intros f v Hnin Hin Hget''.
+      edestruct Hfun' as
+          [rhof1 [B1 [f1 [rhof2 [B2 [f2 [tau'' [t'' [Heq [Hget' Hcc']]]]]]]]]]; eauto.
+      subst. repeat eexists; eauto.
+      rewrite M.gso. eassumption. 
+      intros Hc. subst; eapply Hd; eauto.
+    + eapply env_inv_extend_r. now intros Heq; subst; eapply Hd; eauto.
+      eassumption.
+    + intros v Hget. eexists. rewrite M.gss. split; eauto.
+      edestruct Hfun as [tau' [t' [vs' [Hget' Hfun']]]].
+      rewrite Hget' in H10; inv H10.
+      edestruct Hfun' as
+          [rhof1 [B1 [f1 [rhof2 [B2 [f2 [tau'' [t'' [Heq [Hget'' Hcc']]]]]]]]]]; eauto.
+      subst. rewrite Hget'' in H11. inv H11.
+      now rewrite cc_approx_val_eq in *.
+  - inv Hctx. inv H12.
+    repeat split; eauto.
+    + intros Hc. inv Hc. eauto.
+    + eapply cc_approx_env_P_set_not_in_P_r. eassumption.
+      constructor. intros y Hc. eapply Hd.
+      inv Hc. inv H4. eauto. 
+    + edestruct Hfun as [tau' [t' [vs' [Hget Hfun']]]].
+      rewrite Hget in H10; inv H10.
+      do 3 eexists. rewrite M.gso; [ | now intros Heq; subst; eapply Hd; eauto ].
+      split; eauto. intros f v' Hnin Hin Hget''.
+      edestruct Hfun' as
+          [rhof1 [B1 [f1 [rhof2 [B2 [f2 [tau'' [t'' [Heq [Hget' Hcc']]]]]]]]]]; eauto.
+      subst. repeat eexists; eauto.
+      rewrite M.gso. eassumption. 
+      intros Hc. subst; eapply Hd; eauto.
+    + eapply env_inv_extend_r. now intros Heq; subst; eapply Hd; eauto.
+      eassumption.
+    + intros v' Hget. eexists. rewrite M.gss. split; eauto.
+      edestruct Henv as [tau' [t' [vs' [Hget' Henv']]]].
+      rewrite Hget' in H10; inv H10.
+      edestruct Henv' as [v'' [Hnth Hcc']]; eauto.
+      rewrite H11 in Hnth. now inv Hnth.
+Qed.
+
+Lemma ctx_to_rho_comp_ctx C C1 C2 rho rho' :
+  ctx_to_rho C rho rho' ->
+  comp_ctx C1 C2 C ->
+  exists rho'',
+    ctx_to_rho C1 rho rho'' /\
+    ctx_to_rho C2 rho'' rho'.
+Proof.
+  intros Hctx. revert C1 C2.
+  induction Hctx; intros C1 C2 Hcomp.
+  - inv Hcomp. eexists; split; constructor.
+  - inv Hcomp.
+    + edestruct IHHctx as [rho'' [H1 H2]].
+      constructor. inv H1.
+      eexists; split. constructor.
+      econstructor; eauto.
+    + edestruct IHHctx as [rho'' [H1 H2]]. eassumption.
+      eexists; split. econstructor; eauto.
+      eassumption.
+  - inv Hcomp.
+    + edestruct IHHctx as [rho'' [H1 H2]].
+      constructor. inv H1.
+      eexists; split. constructor.
+      econstructor; eauto.
+    + edestruct IHHctx as [rho'' [H1 H2]]. eassumption.
+      eexists; split. econstructor; eauto.
+      eassumption.
+Qed.
+
+Lemma ctx_to_rho_comp_ctx_f C1 C2 rho1 rho2 rho3 :
+  ctx_to_rho C1 rho1 rho2 ->
+  ctx_to_rho C2 rho2 rho3 ->
+  ctx_to_rho (comp_ctx_f C1 C2) rho1 rho3.
+Proof.
+  revert C2 rho1 rho2 rho3.
+  induction C1; intros C2 rho1 rho2 rho3 Hctx1 GHctx2; inv Hctx1.
+  - eassumption.
+  - simpl; econstructor; eauto. 
+  - simpl; econstructor; eauto.
+Qed.
+
+Lemma project_var_free_set_Included Scope Funs Γ FVs x x' C S S' :
+  project_var Scope Funs Γ FVs S x x' C S' ->
+  Included _ S' S.
+Proof.
+  intros Hproj. inv Hproj.
+  - now apply Included_refl.
+  - now apply Subset_Setminus.
+  - now apply Subset_Setminus.
+Qed.
+
+Lemma project_vars_free_set_Included Scope Funs Γ FVs xs xs' C S S' :
+  project_vars Scope Funs Γ FVs S xs xs' C S' ->
+  Included _ S' S.
+Proof.
+  intros Hproj. induction Hproj.
+  - now apply Included_refl.
+  - eapply Included_trans. eassumption.
+    eapply project_var_free_set_Included. eassumption. 
+Qed.
+
+Lemma project_var_get Scope Funs Γ FVs S1 x x' C1 S2 rho1 rho2 y:
+  project_var Scope Funs Γ FVs S1 x x' C1 S2 ->
+  ctx_to_rho C1 rho1 rho2 ->
+  ~ In _ S1 y ->
+  M.get y rho1 = M.get y rho2. 
+Proof.
+  intros Hvar Hctx Hin. inv Hvar.
+  - inv Hctx. reflexivity.
+  - inv Hctx. inv H12.
+    destruct (Coqlib.peq y x'); subst.
+    contradiction.
+    now rewrite M.gso.
+  - inv Hctx. inv H12.
+    destruct (Coqlib.peq y x'); subst.
+    contradiction.
+    now rewrite M.gso.
+Qed.    
+
+Lemma project_vars_get Scope Funs Γ FVs S1 xs xs' C1 S2 rho1 rho2 y:
+  project_vars Scope Funs Γ FVs S1 xs xs' C1 S2 ->
+  ctx_to_rho C1 rho1 rho2 ->
+  ~ In _ S1 y ->
+  M.get y rho1 = M.get y rho2. 
+Proof.
+  revert Scope Funs Γ FVs S1 xs' C1 S2 rho1 rho2 y.
+  induction xs; intros Scope Funs Γ FVs S1 xs' C1 S2 rho1 rho2 y Hproj Hctx Hnin.
+  - inv Hproj. inv Hctx. reflexivity.
+  - inv Hproj.  
+    edestruct ctx_to_rho_comp_ctx as [rho'' [Hctx1 Hctx2]]; eauto.
+    rewrite <- comp_ctx_f_correct. reflexivity.
+    eapply project_var_get in Hctx1; eauto. 
+    eapply IHxs in Hctx2; eauto.
+    rewrite Hctx1, <- Hctx2. reflexivity.
+    inv H6. eauto.
+    intros Hc. inv Hc. eauto.
+    intros Hc. inv Hc. eauto.
+Qed.
+
+Lemma project_var_getlist Scope Funs Γ FVs S1 x x' C1 S2 rho1 rho2 ys :
+  project_var Scope Funs Γ FVs S1 x x' C1 S2 ->
+  ctx_to_rho C1 rho1 rho2 ->
+  Disjoint _ S1 (FromList ys) ->
+  getlist ys rho1 = getlist ys rho2. 
+Proof.
+  revert rho1 rho2; induction ys; intros rho1 rho2  Hproj Hctx Hnin.
+  - reflexivity. 
+  - simpl.
+    rewrite FromList_cons in Hnin. eapply Disjoint_sym in Hnin. 
+    erewrite project_var_get; eauto.
+    erewrite IHys; eauto.
+    eapply Disjoint_sym. eapply Disjoint_Union_r. eassumption.
+    intros Hc. eapply Hnin. eauto.
+Qed.        
+
+
+Lemma project_vars_getlist Scope Funs Γ FVs S1 xs xs' C1 S2 rho1 rho2 ys :
+  project_vars Scope Funs Γ FVs S1 xs xs' C1 S2 ->
+  ctx_to_rho C1 rho1 rho2 ->
+  Disjoint _ S1 (FromList ys) ->
+  getlist ys rho1 = getlist ys rho2. 
+Proof.
+  revert rho1 rho2; induction ys; intros rho1 rho2  Hproj Hctx Hnin.
+  - reflexivity. 
+  - simpl.
+    rewrite FromList_cons in Hnin. eapply Disjoint_sym in Hnin. 
+    erewrite project_vars_get; eauto.
+    erewrite IHys; eauto.
+    eapply Disjoint_sym. eapply Disjoint_Union_r. eassumption.
+    intros Hc. eapply Hnin. eauto.
+Qed.        
+
+Lemma project_vars_correct k rho1 rho2 rho2'
+      Scope Funs Γ FVs xs xs' C S S'  :
+  project_vars Scope Funs Γ FVs S xs xs' C S' ->
+  cc_approx_env_P Scope k rho1 rho2 ->
+  Fun_inv k rho1 rho2 Scope Funs Γ ->
+  env_inv k rho1 rho2 Scope Funs Γ FVs ->
+  ctx_to_rho C rho2 rho2' ->
+  Disjoint _ S (Union var Scope
+                      (Union var Funs
+                             (Union var (FromList FVs) (Singleton var Γ)))) ->
+  cc_approx_env_P Scope k rho1 rho2' /\
+  Fun_inv k rho1 rho2' Scope Funs Γ /\
+  env_inv k rho1 rho2' Scope Funs Γ FVs /\
+  (forall vs,
+     getlist xs rho1 = Some vs ->
+     exists vs', getlist xs' rho2' = Some vs' /\
+            Forall2 (cc_approx_val k) vs vs').
+Proof.
+  revert k rho1 rho2 rho2' Scope Funs Γ FVs xs' C S.
+  induction xs;
+    intros k rho1 rho2 rho2' Scope Funs Γ FVs xs' C S Hproj Hcc Hfun Henv Hctx Hd.
+  - inv Hproj. inv Hctx. repeat split; eauto. 
+    eexists. split. reflexivity. 
+    inv H. now constructor. 
+  - inv Hproj.
+    edestruct ctx_to_rho_comp_ctx as [rho'' [Hctx1 Hctx2]]; eauto.
+    rewrite <- comp_ctx_f_correct. reflexivity.
+    eapply project_var_correct in Hctx1; eauto.
+    destruct Hctx1 as [Hnin [Hcc1 [Hfun1 [Henv1 Hcc_var]]]].
+    edestruct IHxs as [Hcc2 [Hfun2 [Henv2 Hyp]]]; eauto;
+    [ eapply Disjoint_Included_l; [| eassumption ];
+      eapply project_var_free_set_Included; eassumption |].
+    repeat split; eauto. intros vs Hget. 
+    simpl in Hget. destruct (M.get a rho1) eqn:Hget'; try discriminate. 
+    destruct (getlist xs rho1) eqn:Hgetlist; try discriminate.
+    inv Hget. edestruct Hyp as [vs' [Hgetlist' Hall]]; [ reflexivity |].
+    edestruct Hcc_var as [v' [Hget''' Hcc''']]; eauto.
+    eexists. split; eauto. simpl. rewrite Hgetlist'. 
+    erewrite <- project_vars_get; eauto. rewrite Hget'''. reflexivity.
+Qed.
+
+Lemma ctx_to_rho_cc_approx_exp k rho1 rho2 rho2' C e e' :
+  ctx_to_rho C rho2 rho2' ->
+  cc_approx_exp k (e, rho1) (e', rho2') ->
+  cc_approx_exp k (e, rho1) (C |[ e' ]|, rho2).
+Proof.  
+  intros Hctx Hcc. induction Hctx.
+  - assumption.
+  - intros v1 c1 Hleq1 Hstep1.
+    edestruct IHHctx as [v2 [c2 [Hstep2 Hcc2]]]; eauto.
+    repeat eexists; eauto.
+    simpl. econstructor; eauto.
+  - intros v1' c1 Hleq1 Hstep1.
+    edestruct IHHctx as [v2' [c2 [Hstep2 Hcc2]]]; eauto.
+    repeat eexists; eauto.
+    simpl. econstructor; eauto. simpl.
+    rewrite H, H0. reflexivity.
+Qed.
+
+Lemma Union_Included {A} S1 S2 S :
+  Included A S1 S ->
+  Included A S2 S ->
+  Included A (Union A S1 S2) S.
+Proof. 
+  intros H1 H2 x Hin; inv Hin; eauto.
+Qed.
+
+Lemma Singleton_Included {A} x S :
+  In A S x ->
+  Included A (Singleton A x) S.
+Proof. 
+  intros H x' Hin; inv Hin; eauto.
+Qed.
+
+Lemma project_var_In_Union Scope Funs Γ FVs S x x' C S' :
+  project_var Scope Funs Γ FVs S x x' C S' ->
+  In _ (Union var Scope (Union var Funs (FromList FVs))) x.
+Proof.
+  intros Hvar. inv Hvar; eauto.
+  right; right. eapply nthN_In. eassumption.
+Qed.
+
+Lemma project_vars_In_Union Scope Funs Γ FVs S xs xs' C S' :
+  project_vars Scope Funs Γ FVs S xs xs' C S' ->
+  Included var (FromList xs) (Union var Scope (Union var Funs (FromList FVs))).
+Proof.
+  intros Hvar. induction Hvar; eauto.
+  - rewrite FromList_nil. now apply Included_Empty_set.
+  - rewrite FromList_cons.
+    eapply Union_Included; [| eassumption ].
+    eapply Singleton_Included. eapply project_var_In_Union.
+    eassumption.
+Qed.
+
+Lemma project_var_ctx_to_rho Scope Funs Γ FVs x x' C S S' v1 k rho1 rho2 :
+  project_var Scope Funs Γ FVs S x x' C S' ->
+  env_inv k rho1 rho2 Scope Funs Γ FVs ->
+  Fun_inv k rho1 rho2 Scope Funs Γ ->
+  M.get x rho1 = Some v1 ->
+  exists rho2', ctx_to_rho C rho2 rho2'.
+Proof. 
+  intros Hproj [t' [tau' [vs' [Hget3' Henv]]]]
+         [t [tau [vs [Hget3 Hfun]]]] Hget1; inv Hproj.
+  - eexists; econstructor; eauto.
+  - edestruct Hfun as
+        [rho1' [B1 [f1 [rho2' [B2 [f2 [tau2 [t2 [Heq' [Hget2 Happrox2]]]]]]]]]]; eauto.
+    eexists; econstructor; eauto. constructor.
+  - rewrite Hget3 in Hget3'; inv Hget3'.
+    edestruct Henv as [y [Hnth Hcc]]; eauto.
+    eexists. econstructor; eauto. constructor. 
+Qed.
+
+Lemma project_var_not_In Scope Funs Γ FVs S x x' C S' :
+  Disjoint _ S (Union var Scope
+                      (Union var Funs
+                             (Union var (FromList FVs) (Singleton var Γ)))) ->
+      
+  project_var Scope Funs Γ FVs S x x' C S' ->
+  ~ In _ S x.
+Proof.
+  intros Hd  Hproj. inv Hproj; intros Hin; try now eapply Hd; eauto.
+  eapply nthN_In in H1. eapply Hd. eauto.
+Qed.
+
+Lemma project_vars_Disjoint Scope Funs Γ FVs S xs xs' C S' :
+  Disjoint _ S (Union var Scope
+                      (Union var Funs
+                             (Union var (FromList FVs) (Singleton var Γ)))) ->      
+  project_vars Scope Funs Γ FVs S xs xs' C S' ->
+  Disjoint _ S (FromList xs).
+Proof.
+  revert xs' C S S'; induction xs; intros xs' C S S' Hd Hproj.
+  - rewrite FromList_nil. now eapply Disjoint_Empty_set_r.
+  - inv Hproj. rewrite FromList_cons.
+    eapply Disjoint_sym; eapply Disjoint_Union; eapply Disjoint_sym.
+    eapply Disjoint_Singleton. eapply project_var_not_In; eauto.
+    inv H6.
+    + eapply IHxs; [| eassumption ]. eauto.
+    + assert (Hd1 : Disjoint _ (Setminus var S (Singleton var y')) (FromList xs)).
+      { eapply IHxs; eauto.
+        eapply Disjoint_Included_l; [| eassumption ].
+        eapply Subset_Setminus. }
+      eapply Disjoint_Included_l with (s3 := Union _ S (Singleton _ y')).
+      now apply Included_Union_l.
+      rewrite (@Union_Setminus _ _ _ _).
+      eapply Disjoint_Union; eauto.
+      eapply project_vars_In_Union in H10. 
+      constructor. intros x Hc. inv Hc.
+      inv H2. eapply Hd. constructor.
+      eassumption. eapply H10 in H3. inv H3; eauto.
+      inv H2; eauto.
+    + assert (Hd1 : Disjoint _ (Setminus var S (Singleton var y')) (FromList xs)).
+      { eapply IHxs; eauto.
+        eapply Disjoint_Included_l; [| eassumption ].
+        eapply Subset_Setminus. }
+      eapply Disjoint_Included_l with (s3 := Union _ S (Singleton _ y')).
+      now apply Included_Union_l.
+      rewrite (@Union_Setminus _ _ _ _).
+      eapply Disjoint_Union; eauto.
+      eapply project_vars_In_Union in H10.  
+      constructor. intros x Hc. inv Hc.
+      inv H3. eapply Hd. constructor.
+      eassumption. eapply H10 in H4. inv H4; eauto.
+      inv H3; eauto.
+Qed.
+
+Lemma project_vars_ctx_to_rho Scope Funs Γ FVs xs xs' C S S' vs1 k rho1 rho2 :
+  Disjoint _ S (Union var Scope
+                      (Union var Funs
+                             (Union var (FromList FVs) (Singleton var Γ)))) ->
+  project_vars Scope Funs Γ FVs S xs xs' C S' ->
+  Fun_inv k rho1 rho2 Scope Funs Γ ->
+  env_inv k rho1 rho2 Scope Funs Γ FVs ->
+  getlist xs rho1 = Some vs1 ->
+  exists rho2', ctx_to_rho C rho2 rho2'.
+Proof. 
+  intros HD Hvars Hfun [tau [t [vs [Hget Henv]]]].
+  assert (HD' := Hvars).
+  apply project_vars_Disjoint in HD'; [ | eassumption ]. 
+  revert Scope Funs Γ FVs xs' C S S' vs1 tau t vs k
+         rho1 rho2  HD HD' Hvars Hfun Hget Henv. 
+  induction xs;
+    intros Scope Funs Γ FVs xs' C S S' vs1 tau t vs k
+           rho1 rho2 HD  HD' Hvars Hfun Hget Hclo Hgetlist.
+  - inv Hvars. eexists; econstructor; eauto.
+  - inv Hvars. simpl in Hgetlist.
+    destruct (M.get a rho1) eqn:Hgeta1; try discriminate. 
+    destruct (getlist xs rho1) eqn:Hgetlist1; try discriminate.
+    edestruct project_var_ctx_to_rho with (rho1 := rho1) as [rho2' Hctx1]; eauto.
+    now do 3 eexists; split; eauto. 
+    edestruct IHxs with (rho2 := rho2') as [rho2'' Hctx2];
+      [|  | eassumption | | | eassumption | eassumption | ].
+    + eapply Disjoint_Included_l; [| eassumption ].
+      eapply project_var_free_set_Included. eassumption.
+    + rewrite FromList_cons in HD'.
+      eapply Disjoint_Included_l.
+      * eapply project_var_free_set_Included. eassumption.
+      * eapply Disjoint_Included_r; [| eassumption ].
+        eapply Included_Union_r.
+    + do 3 eexists; split.
+      erewrite <- project_var_get; eauto.
+      intros Hin. eapply HD. eauto.
+      intros f v' Hnin Hin Hgetv'.
+      edestruct Hfun as [tau1 [t1 [vs' [Hget1 Hfun']]]].
+      rewrite Hget1 in Hget. inv Hget.
+      edestruct Hfun' as
+          [rho1f' [B1 [f1 [rho2f' [B2 [f2 [tau2 [t2 [Heq' [Hget2 Happrox2]]]]]]]]]];
+        eauto.
+      subst. repeat eexists; eauto.
+      erewrite <- project_var_get; eauto. 
+      intros Hin'. eapply HD. eauto.
+    + erewrite <- project_var_get; eauto. 
+      intros Hin. eapply HD. eauto.
+    + exists rho2''. eapply ctx_to_rho_comp_ctx_f; eassumption.
+Qed.
+
+(* Lemma bstep_e_ctx_app rho C e1 e2 v c : *)
+(*   (forall rho v c, bstep_e rho e1 v c -> bstep_e rho e2 v c) -> *)
+(*   bstep_e rho (C |[ e1 ]|) v c-> *)
+(*   bstep_e rho (C |[ e2 ]|) v c. *)
+(* Proof.   *)
+(*   revert rho e1 e2 v c. *)
+(*   induction C; eauto; intros rho e1 e2 v' c Hyp Hstep; inv Hstep; try (now econstructor; eauto). *)
+(*   - apply findtag_append_spec in H3. *)
+(*     edestruct H3 as [Hfind | [Hfind Hnin]]. *)
+(*     + simpl. econstructor; eauto. *)
+(*       now eapply findtag_append_Some.  *)
+(*     + simpl in Hfind. edestruct (M.elt_eq t t0) eqn:Heq; subst. *)
+(*       * inv Hfind. simpl; econstructor; [| | eapply IHC ]; eauto. *)
+(*         rewrite findtag_append_not_In; [| eassumption ]. *)
+(*         simpl; now rewrite Heq. *)
+(*       * inv Hfind. simpl; econstructor; eauto. *)
+(*         rewrite findtag_append_not_In; [| eassumption ]. *)
+(*         simpl; now rewrite Heq. *)
+(*   - admit. *)
+(* Admitted. *)
+
+Lemma Complement_Disjoint {A} S1 S2 :
+  Included A S1 S2 ->
+  Disjoint A (Complement _ S2) S1.
+Proof.   
+  intros Hin. constructor. intros x Hin'.
+  inv Hin'. eauto.
+Qed.
+
+                     
 Lemma closure_conversion_correct k rho rho' e e' Scope Funs Γ FVs :
   cc_approx_env_P Scope k rho rho' ->
   ~ In _ (bound_var e) Γ ->
@@ -441,9 +906,37 @@ Proof.
   revert k e rho rho' e' Scope Funs Γ FVs.
   induction k as [k IHk] using lt_wf_rec1.
   induction e using exp_ind';
-    intros rho rho' e' Scope Funs Γ FVs Happrox Hnin Hfun Henv Hcc.
-  - (* Case Econstr. Induction on l and the similar to Eproj *) 
-    admit.
+    intros rho1 rho2 e' Scope Funs Γ FVs Happrox Hnin Hfun Henv Hcc.
+  - (* Case Econstr. Induction on l and then similar to Eproj *)
+    inv Hcc.
+    intros v1 c1 Hleq Hstep. inv Hstep.
+    edestruct project_vars_ctx_to_rho as [rho2' Hto_rho]; eauto.
+    eapply Complement_Disjoint. now apply Included_refl.
+    edestruct project_vars_correct as [Happ [Hfun' [Henv' Hvar]]]; eauto.
+    eapply Complement_Disjoint. now apply Included_refl.
+    edestruct Hvar as [v' [Hget' Happ']]; eauto.
+    eapply ctx_to_rho_cc_approx_exp; eauto.
+    intros v1' c1' Hleq' Hstep'. eapply bstep_e_deterministic in H11; eauto.
+    inv H11.
+    edestruct IHe as [v2'' [c2 [Hstep2 Happrox2]]];
+        [| now eauto | | | eassumption | eassumption | eassumption | ]. 
+    + eapply cc_approx_env_P_extend with (v2 := Vconstr tau' t0 v').
+      rewrite Setminus_Union_distr,
+      Setminus_Empty_set, Union_Empty_set_r. 
+      eapply cc_approx_env_P_antimon; [ eassumption |].
+      eapply Setminus_Included. now apply Included_refl.
+      rewrite cc_approx_val_eq. constructor; eauto.
+      now eapply Forall2_Forall2_asym_included.
+    + eapply Fun_inv_set_In_Scope_l. now eauto.
+      eapply Fun_inv_set_In_Scope_r_not_Γ. now eauto.
+      intros Heq; subst. now eauto.
+      eapply Fun_inv_mon; [ | now eauto ].
+      eapply Included_Union_r.
+    + eapply env_inv_extend_In_Scope_l. now constructor.
+      eapply env_inv_extend_r. intros Hc. eapply Hnin.
+      subst. now eauto. now eapply env_inv_extend_Scope.
+    + repeat eexists; [| eassumption ].
+      econstructor; eauto.
   - (* Case [Ecase x []] *)
     inv Hcc. destruct pats'; [| now inv H7 ].
     intros v1 c1 Hleq Hstep. inv Hstep. inv H3. 
@@ -464,7 +957,7 @@ Proof.
         econstructor; eauto. simpl. now rewrite Heq.
       - edestruct Hfun as [tau1 [t1 [vs1 [Hget1 Hfun']]]].
         edestruct Hfun' as
-            [rho1 [B1 [f1 [rho2 [B2 [f2 [tau2 [t2 [Heq' [Hget2 Happrox2]]]]]]]]]];
+            [rho1' [B1 [f1 [rho2' [B2 [f2 [tau2 [t2 [Heq' [Hget2 Happrox2]]]]]]]]]];
           [| | now apply H1 | ]; eauto. congruence.
       - edestruct Henv as [tau1 [t1 [vs1 [Hget Henv']]]]; eauto.
         edestruct Henv' as [v' [Hnth' Happrox2]]; eauto.
@@ -495,7 +988,7 @@ Proof.
         now rewrite Heq. 
       - edestruct Hfun as [tau1 [t1 [vs1 [Hget1 Hfun']]]].
         edestruct Hfun' as
-            [rho1 [B1 [f1 [rho2 [B2 [f2 [tau2 [t2 [Heq' [Hget2 Happrox2]]]]]]]]]];
+            [rho1' [B1 [f1 [rho2' [B2 [f2 [tau2 [t2 [Heq' [Hget2 Happrox2]]]]]]]]]];
           [| | now apply H1 | ]; eauto. congruence.
       - edestruct Henv as [tau1 [t1 [vs1 [Hget Henv']]]]; eauto.
         edestruct Henv' as [v' [Hnth' Happrox2]]; eauto.
@@ -511,64 +1004,125 @@ Proof.
         econstructor; eauto. simpl.
         rewrite M.gss in H10. inv H10. now rewrite Heq. }
   - (* Case Eproj *)
-    inv Hcc. inv H9.
-    + intros v1 c1 Hleq Hstep. inv Hstep.
-      edestruct Happrox as [vcon [Hget' Happrox2]]; eauto.
-      rewrite cc_approx_val_eq in Happrox2.
-      destruct vcon; try contradiction. inv Happrox2.
-      edestruct (@Forall2_asym_nthN val) as [v0' [Hnth' Happrox3]]; eauto.
-      edestruct IHe as [v2 [c2 [Hstep2 Happrox2]]];
-        [| now eauto | | | eassumption | eassumption | eassumption | ].
-      * eapply cc_approx_env_P_extend; [| eassumption ].
-        rewrite Setminus_Union_distr,
-        Setminus_Empty_set, Union_Empty_set_r. 
-        eapply cc_approx_env_P_antimon; [ eassumption |].
-        eapply Setminus_Included. now apply Included_refl.      
-      * eapply Fun_inv_set_In_Scope_l. now eauto.
-        eapply Fun_inv_set_In_Scope_r_not_Γ. now eauto.
-        intros Heq; subst. now eauto.
-        eapply Fun_inv_mon; [ | now eauto ].
-        eapply Included_Union_r.
-      * eapply env_inv_extend_In_Scope_l. now constructor.
-        eapply env_inv_extend_r. intros Hc. eapply Hnin.
-        subst. now eauto. now eapply env_inv_extend_Scope.
-      * repeat eexists; [| eassumption ].
-        econstructor; eauto.
-    + intros v1 c1 Hleq Hstep. inv Hstep. simpl.
-      edestruct Hfun as [tau1 [t1 [vs1 [Hget1 Hfun']]]].
-      edestruct Hfun' as
-          [rho1 [B1 [f1 [rho2 [B2 [f2 [tau2 [t2 [Heq [Hget2 Happrox2]]]]]]]]]]; [| | now apply H11 | ];
-      eauto.
-      congruence.
-    + simpl. intros v1 c1 Hleq Hstep. inv Hstep.
-      edestruct Henv as [tau1 [t1 [vs1 [Hget Henv']]]]; eauto.
-      edestruct Henv' as [v' [Hnth' Happrox2]]; eauto.
-      rewrite cc_approx_val_eq in Happrox2.
-      destruct v'; try contradiction. inv Happrox2.
-      edestruct (@Forall2_asym_nthN val) as [v0' [Hnth'' Happrox3]]; eauto.
-      edestruct IHe as [v2' [c2 [Hstep2 Happrox2]]];
-        [ | now eauto | | | eassumption | eassumption | eassumption |
-          repeat eexists; [| eassumption ]; econstructor; eauto;
-          econstructor; eauto; rewrite M.gss; reflexivity ].
-      * eapply cc_approx_env_P_extend; [| eassumption ].
-        rewrite Setminus_Union_distr,
-        Setminus_Empty_set, Union_Empty_set_r.
-        eapply cc_approx_env_P_not_in_P_r.
-        eapply cc_approx_env_P_antimon; eauto. eapply Setminus_Included.
-        now eapply Included_refl. intros Hin. inv Hin. eapply H2. eauto. 
-      * eapply Fun_inv_set_In_Scope_l. now eauto.
-        eapply Fun_inv_set_In_Scope_r_not_Γ. now eauto.
-        intros Heq; subst. now eauto.
-        eapply Fun_inv_set_not_In_Funs_r_not_Γ. now eauto.
-        intros Heq; subst. now eauto.
-        eapply Fun_inv_mon; [ | now eauto ]. eapply Included_Union_r.
-      * eapply env_inv_extend_In_Scope_l. now constructor.
-        eapply env_inv_extend_r. intros Hc. subst. now eauto.
-        eapply env_inv_extend_r. intros Hc. subst. now eauto.
-        now apply env_inv_extend_Scope. 
-  - (* Case Efun -- the hardest one! *)
     inv Hcc.
+    intros v1 c1 Hleq Hstep. inv Hstep.
+    edestruct project_var_ctx_to_rho as [rho2' Hto_rho]; eauto.
+    edestruct project_var_correct as [Hnin' [Happ [Hfun' [Henv' Hvar]]]]; eauto.
+    eapply Complement_Disjoint. now apply Included_refl.
+    edestruct Hvar as [v' [Hget' Happ']]; eauto.
+    rewrite cc_approx_val_eq in Happ'. destruct v'; try contradiction.
+    inv Happ'. eapply ctx_to_rho_cc_approx_exp; eauto.
+    intros v1' c1' Hleq' Hstep'. eapply bstep_e_deterministic in H11; eauto.
+    inv H11. edestruct (@Forall2_asym_nthN val) as [v2' [Hnth2 Happ2]]; eauto.
+    edestruct IHe as [v2'' [c2 [Hstep2 Happrox2]]];
+        [| now eauto | | | eassumption | eassumption | eassumption | ]. 
+    + eapply cc_approx_env_P_extend; [| eassumption ].
+      rewrite Setminus_Union_distr,
+      Setminus_Empty_set, Union_Empty_set_r. 
+      eapply cc_approx_env_P_antimon; [ eassumption |].
+      eapply Setminus_Included. now apply Included_refl.      
+    + eapply Fun_inv_set_In_Scope_l. now eauto.
+      eapply Fun_inv_set_In_Scope_r_not_Γ. now eauto.
+      intros Heq; subst. now eauto.
+      eapply Fun_inv_mon; [ | now eauto ].
+      eapply Included_Union_r.
+    + eapply env_inv_extend_In_Scope_l. now constructor.
+      eapply env_inv_extend_r. intros Hc. eapply Hnin.
+      subst. now eauto. now eapply env_inv_extend_Scope.
+    + repeat eexists; [| eassumption ].
+      econstructor; eauto.
+  - (* Case Efun -- the hardest one! *) 
+    inv Hcc. 
     (* edestruct Henv as [tau' [t' [vs' [Hget Hclo]]]].  *)
-    eapply closure_conversion_fundefs_correct with
-    (rho := rho) (rho' := rho') in H3; eauto.
+    (* eapply closure_conversion_fundefs_correct with *)
+    (* (rho := rho) (rho' := rho') in H3 ; eauto. *)
+    admit.
+  - (* Case Eapp *)
+    inv Hcc.
+    intros v1 c1 Hleq Hstep. inv Hstep.
+    + edestruct project_vars_ctx_to_rho as [rho2' Hto_rho]; eauto.
+      eapply Complement_Disjoint. now apply Included_refl.      
+      simpl. rewrite H3, H7. reflexivity.
+      edestruct project_vars_correct as [Happ [Hfun' [Henv' Hvar]]]; eauto.
+      eapply Complement_Disjoint. now apply Included_refl.
+      edestruct Hvar as [v' [Hget' Happ']]; eauto.
+      simpl. rewrite H3, H7. reflexivity.
+      simpl in Hget'. destruct (M.get f' rho2') eqn:Hgetf'; try discriminate.
+      destruct (getlist ys' rho2') eqn:Hgetlist'; try discriminate. inv Hget'.
+      inv Happ'. rewrite cc_approx_val_eq in H4. destruct v0; try contradiction.
+      eapply ctx_to_rho_cc_approx_exp with (e := Eapp v l); eauto.
+      * intros v1' c1' Hleq' Hstep'.
+        inv Hstep'. rewrite H3 in H5. inv H5.
+        rewrite H7 in H12; inv H12.
+        admit. (* the relation needs tweaking *)
+        rewrite H3 in H2. congruence.
+      * constructor; eauto.
+    + edestruct project_vars_ctx_to_rho as [rho2' Hto_rho]; eauto.
+      eapply Complement_Disjoint. now apply Included_refl.      
+      simpl. rewrite H2, H3. reflexivity.
+      edestruct project_vars_correct as [Happ [Hfun' [Henv' Hvar]]]; eauto.
+      eapply Complement_Disjoint. now apply Included_refl.
+      edestruct Hvar as [v' [Hget' Happ']]; eauto.
+      simpl. rewrite H2, H3. reflexivity.
+      simpl in Hget'. destruct (M.get f' rho2') eqn:Hgetf'; try discriminate.
+      destruct (getlist ys' rho2') eqn:Hgetlist'; try discriminate. inv Hget'.
+      inv Happ'. rewrite cc_approx_val_eq in H9. destruct v0; try contradiction.
+      eapply ctx_to_rho_cc_approx_exp with (e := Eapp v l); eauto.
+      * intros v1' c1' Hleq' Hstep'.
+        inv Hstep'.
+        { rewrite H3 in H15. inv H15. 
+          rewrite H2 in H10; inv H10. }
+        { rewrite H3 in H10. inv H10. 
+          rewrite H2 in H5; inv H5.
+          destruct l1; try contradiction. destruct v0, l1; try contradiction.
+          destruct v2; try contradiction. simpl in H9.
+          rewrite H13 in H4. inv H4. 
+          rewrite H7 in H15. inv H15. eapply bstep_e_deterministic in H18; eauto. inv H18.
+          assert (Hlen := List_util.Forall2_length _ _ _ H12).
+          edestruct H9 with (vs2 := l0) (j := k - 1)
+            as [t2' [Γ' [xs2 [e2 [rho2'' [Hfind [Hset Hyp]]]]]]]; eauto.
+          edestruct Hyp as [v2' [c2 [Hstep2 Hcc']]]; try eassumption. omega.
+          eapply List_util.Forall2_monotonic; [| eassumption ].
+          intros. eapply cc_approx_val_monotonic. eassumption. omega. omega.
+          repeat eexists; eauto. econstructor. eassumption. reflexivity.
+          econstructor. rewrite M.gso. eassumption. admit.
+          reflexivity.
+          eapply BStep_app_fun. rewrite M.gso. rewrite M.gss. reflexivity.
+          admit. simpl. rewrite M.gss.
+          assert (Ha :
+                    getlist ys'
+                            (M.set env' (Vconstr t4 t5 l2) (M.set f'' (Vfun t3 f v0) rho2')) = Some l0)
+            by admit.
+          rewrite Ha. reflexivity. eassumption.
+          eauto. eassumption. simpl.
+          eapply cc_approx_val_monotonic. eassumption. omega. }
+        * econstructor; eauto. 
+  - inv Hcc.
+    intros v1 c1 Hleq Hstep. inv Hstep.
+    edestruct project_vars_ctx_to_rho as [rho2' Hto_rho]; eauto.
+    eapply Complement_Disjoint. now apply Included_refl.
+    edestruct project_vars_correct as [Happ [Hfun' [Henv' Hvar]]]; eauto.
+    eapply Complement_Disjoint. now apply Included_refl.
+    edestruct Hvar as [v' [Hget' Happ']]; eauto.
+    eapply ctx_to_rho_cc_approx_exp; eauto.
+    intros v1' c1' Hleq' Hstep'. eapply bstep_e_deterministic in H13; eauto.
+    inv H11.
+    edestruct Prim_axiom as [vs' [Hf' Hcc]]; eauto.
+    edestruct IHe as [v2'' [c2 [Hstep2 Happrox2]]];
+        [| now eauto | | | eassumption | eassumption | eassumption | ]. 
+    + eapply cc_approx_env_P_extend; [| eassumption ].
+      rewrite Setminus_Union_distr,
+      Setminus_Empty_set, Union_Empty_set_r. 
+      eapply cc_approx_env_P_antimon; [ eassumption |].
+      eapply Setminus_Included. now apply Included_refl.
+    + eapply Fun_inv_set_In_Scope_l. now eauto.
+      eapply Fun_inv_set_In_Scope_r_not_Γ. now eauto.
+      intros Heq; subst. now eauto.
+      eapply Fun_inv_mon; [ | now eauto ].
+      eapply Included_Union_r.
+    + eapply env_inv_extend_In_Scope_l. now constructor.
+      eapply env_inv_extend_r. intros Hc. eapply Hnin.
+      subst. now eauto. now eapply env_inv_extend_Scope.
+    + repeat eexists; [| eassumption ].
+      econstructor; eauto.
 Abort.
